Updated structure
Updated structure of DNFP proof. Splitted it up in multiple files

Monad_Play Around/DNFP/Dutch_National_Flag_Monad.thy
@@ -1,105 +1,14 @@
 theory Dutch_National_Flag_Monad
 imports 
-  Main
-  "../State_Monad_HL"
-  "HOL-Library.Multiset"
+  "Dutch_National_Flag_Monad_Definitions_Lemmas"
 begin
 
-text\<open>Monad definiti.ons to encode and extract data from the monad\<close>
-datatype color = red | white | blue
-
-type_synonym 'a array = "'a list"
-
-
-section\<open>Monad definitions\<close>
-record env = 
-  high :: "nat"
-  low  :: "nat"
-  i    :: "nat"
-  xs   :: "nat array"
-  
-subsection\<open>update functions\<close>
-definition high_Env:: "env \<Rightarrow> nat \<Rightarrow> env" where "high_Env s v = s \<lparr> high := v \<rparr>"
-definition low_Env:: "env \<Rightarrow> nat \<Rightarrow> env" where "low_Env s v = s \<lparr> low := v \<rparr>"
-definition i_Env:: "env \<Rightarrow> nat \<Rightarrow> env" where "i_Env s v = s \<lparr> i := v \<rparr>"
-definition xs_Env:: "env \<Rightarrow> nat array  \<Rightarrow> env" where "xs_Env s v = s \<lparr> xs := v \<rparr>"
-
-theorem put_high_rule: "spec (\<lambda>x. p () (x \<lparr> high := v \<rparr>)) (put high_Env v) p"
-  by (simp add: spec_def put_def get_state_def put_state_def high_Env_def)
-
-theorem put_low_rule: "spec (\<lambda>x. p () (x \<lparr> low := v \<rparr>)) (put low_Env v) p"
-  by (simp add: spec_def put_def get_state_def put_state_def low_Env_def)
-
-theorem put_i_rule: "spec (\<lambda>x. p () (x \<lparr> i := v \<rparr>)) (put i_Env v) p"
-  by (simp add: spec_def put_def get_state_def put_state_def i_Env_def)
-
-theorem put_xs_rule: "spec (\<lambda>x. p () (x \<lparr> xs := v \<rparr>)) (put xs_Env v) p"
-  by (simp add: spec_def put_def get_state_def put_state_def xs_Env_def)
 
 section\<open>DNFP\<close>
-
-definition swap:: "'a array \<Rightarrow> nat \<Rightarrow> nat \<Rightarrow> 'a array" where
-"swap l x y \<equiv> (if x < length l \<and> y < length l then l[x := l!y, y := l!x] else l)"
-
-lemma length_swap: "length(swap l x y) = length l"
-  by(simp add: swap_def)
-
-lemma distinct_swap[simp]:
-  "distinct(swap l x y) = distinct l"
-  by(simp add: swap_def)
-
-lemma mset_swap: "mset (swap l x y) = mset l"
-  by (simp add: swap_def mset_swap)
-
-value\<open>swap [a,b,c,d,e] 0 4 = [e,b,c,d,a]\<close>
-
-text\<open>Get i and get low seems not to be necessary\<close>
-definition inc_lowbound where
-"inc_lowbound \<equiv> do{
-                  (l, s, j) \<leftarrow> get (\<lambda>e. (low e, xs e, i e));  
-                  put xs_Env (swap s j l);
-                  j \<leftarrow> get i;                                   
-                  put i_Env (Suc j);
-                  l \<leftarrow> get low;  
-                  put low_Env (Suc l)
-                }"
-
-definition dec_highbound where
-"dec_highbound \<equiv> do{
-                    h \<leftarrow> get high;
-                    put high_Env (h - 1);
-                    (s, j, h) \<leftarrow> get (\<lambda>e. (xs e, i e, high e));
-                    put xs_Env (swap s j h)
-                }"
-
-definition inc_index where
-"inc_index \<equiv> do{
-                  j \<leftarrow> get i;
-                  put i_Env (Suc j)
-                }"
-
-definition loop_update_action where
-"loop_update_action \<equiv> 
-  do{
-    (s, j) \<leftarrow> get (\<lambda>e. (xs e, i e));
-    (if s!j < 1 then do {
-      inc_lowbound
-    } else (if s!j > 1 then do 
-    {
-      dec_highbound
-    }
-   else do {
-      inc_index
-   }))
-  }"
-
-
-
 text\<open>A version using a state monad for storing the list/array that is being sorted\<close>
 fun dnfp_mon:: "nat \<Rightarrow> (env, unit) state" where
   case0:"dnfp_mon 0  = skip"|
-  case1:"dnfp_mon (Suc 0)  = skip"|
-  caseN:"dnfp_mon (Suc n)  = do {
+  caseN:"dnfp_mon (Suc n) = do {
                         (h, j) \<leftarrow> get (\<lambda>e. (high e, i e));
                         (if h > j then do{
                           loop_update_action;
@@ -108,470 +17,8 @@ fun dnfp_mon:: "nat \<Rightarrow> (env, unit) state" where
                        else skip
                       )}"
 
-
-definition init_env:: "nat array \<Rightarrow> env" where
-  "init_env l \<equiv> \<lparr>high = (length l),            low = 0,
-                 i = 0,                         xs = l\<rparr>"
-
-definition init_state_env:: "nat array \<Rightarrow> (env, unit) state" where
-  "init_state_env l \<equiv> State (\<lambda>x. ((),init_env l))"
-
-definition mk_rec:: "nat array \<Rightarrow>nat \<Rightarrow> nat \<Rightarrow> nat \<Rightarrow> env" where
-"mk_rec arr l j h \<equiv> \<lparr>high = h,            low = l,
-                     i = j,               xs = arr\<rparr>"
-
-value \<open>snd(run_state (dnfp_mon 5) (init_env [0,2,2,1,2]))\<close>
-value \<open>snd(run_state (dnfp_mon 9) (init_env [0,2,2,0,1,0,2,1,2]))\<close>
-value \<open>snd(run_state (dnfp_mon 3)(init_env [2,1,0]))\<close>
-
-value \<open>sorted(xs(snd(run_state (dnfp_mon 5) (init_env[0,2,2,1,2]))))\<close>
-value \<open>sorted(xs(snd(run_state (dnfp_mon 9) (init_env[0,2,2,0,1,0,2,1,2]))))\<close>
-value \<open>sorted(xs(snd(run_state (dnfp_mon 3) (init_env[2,1,0]))))\<close>
-
-section\<open>Definiton of all the Pre and postconditions\<close>
-
-subsection\<open>The invariants are taken from https://en.wikipedia.org/wiki/Dutch_national_flag_problem\<close>
-definition low_invariant_is_0 where
-"low_invariant_is_0 arr l \<equiv> (\<forall>x. x < l \<longrightarrow> arr!x = 0)"
-
-definition invariant_low_to_j_is_1 where
-"invariant_low_to_j_is_1 arr l j \<equiv> (\<forall>x. (x \<ge> l \<and> x < j) \<longrightarrow> arr!x = 1)"
-
-definition high_invariant_is_2 where
-"high_invariant_is_2 arr h\<equiv> (\<forall>x. x \<ge> h \<longrightarrow> arr!x = 2)"
-
-definition low_invariant_is_0_Env where
-"low_invariant_is_0_Env e \<equiv> (\<forall>x. x < (low e) \<longrightarrow> (xs e)!x = 0)"
-
-definition invariant_low_to_j_is_1_Env where
-"invariant_low_to_j_is_1_Env e \<equiv> (\<forall>x. (x \<ge> (low e) \<and> x < (i e)) \<longrightarrow> (xs e)!x = 1)"
-
-definition high_invariant_is_2_Env where
-"high_invariant_is_2_Env e\<equiv> (\<forall>x. x \<ge> (high e) \<longrightarrow> (xs e)!x = 2)"
-
-definition invariants_Env:: "env \<Rightarrow> bool" where
-"invariants_Env e \<equiv> high_invariant_is_2_Env e
-              \<and> invariant_low_to_j_is_1_Env e
-              \<and> low_invariant_is_0_Env e"
-
-definition invariants where
-"invariants arr l j h\<equiv> low_invariant_is_0 arr l
-              \<and> invariant_low_to_j_is_1 arr l j
-              \<and> high_invariant_is_2 arr h"
-
-text\<open>This can be used in the other pre and post-conditions for the methods inside loop_update_actions\<close>
-
-subsection\<open>Pre- and Postconditions\<close>
-
-subsubsection\<open>Pre-conditions\<close>
-definition dnfp_pre:: "env \<Rightarrow> env \<Rightarrow> bool" where
-"dnfp_pre e s \<equiv> s = e
-              \<and> high e \<ge> i e
-              \<and> i e \<ge> low e 
-              \<and> length (xs e) \<ge> high e
-              \<and> set (xs e) \<subseteq> {1,2,3}"
-
-definition dnfp_pre_aux:: "env \<Rightarrow> bool" where
-"dnfp_pre_aux e \<equiv> 
-              high e \<ge> i e
-              \<and> i e \<ge> low e 
-              \<and> length (xs e) \<ge> high e
-              \<and> set (xs e) \<subseteq> {1,2,3}"
-
-definition loop_update_action_pre:: "env \<Rightarrow> bool" where
-"loop_update_action_pre e \<equiv> high e > i e
-                             \<and> length (xs e) > (Suc 0)
-                             \<and> length (xs e) \<ge> high e
-                             \<and> low e < high e
-                             \<and> low e \<le> i e
-                             \<and> set (xs e) \<subseteq> {0,1,2}"
-
-definition loop_update_action_pre_aux:: "env \<Rightarrow> env \<Rightarrow> bool" where
-"loop_update_action_pre_aux e s \<equiv> s = e
-                              \<and> loop_update_action_pre e"
-
-definition loop_update_action_inv1 where 
-"loop_update_action_inv1 e \<equiv> loop_update_action_pre e 
-                            \<and> low_invariant_is_0_Env e"
-
-definition loop_update_action_inv2 where 
-"loop_update_action_inv2 e \<equiv> loop_update_action_pre e 
-                              \<and> invariant_low_to_j_is_1_Env e"
-
-definition loop_update_action_inv3 where 
-"loop_update_action_inv3 e \<equiv> loop_update_action_pre e 
-                              \<and> high_invariant_is_2_Env e"
-
-definition loop_update_action_post where
-"loop_update_action_post e e' \<equiv> length (xs e) = length (xs e')
-                                \<and> high e \<ge> high e'
-                                \<and> low e \<le> low e'
-                                \<and> i e \<le> i e'
-                                \<and> high e - i e > high e' - i e'"
-
-definition inc_lowbound_pre:: "env \<Rightarrow> env \<Rightarrow> bool" where 
-"inc_lowbound_pre e s \<equiv> s = e
-                        \<and> loop_update_action_pre s
-                        \<and> (xs s)!(i s) < 1"
-
-definition inc_lowbound_inv1 :: "env \<Rightarrow> bool" where
-"inc_lowbound_inv1 s \<equiv> loop_update_action_pre s
-                        \<and> (xs s)!(i s) < 1
-                        \<and> low_invariant_is_0_Env s"
-
-definition inc_lowbound_inv2 :: "env \<Rightarrow> bool" where
-"inc_lowbound_inv2 s \<equiv> loop_update_action_pre s
-                        \<and> (xs s)!(i s) < 1
-                        \<and> invariant_low_to_j_is_1_Env s"
-
-definition inc_lowbound_inv3 :: "env \<Rightarrow> bool" where
-"inc_lowbound_inv3 s \<equiv> loop_update_action_pre s
-                        \<and> (xs s)!(i s) < 1
-                        \<and> high_invariant_is_2_Env s"
-
-definition dec_highbound_pre where 
-"dec_highbound_pre e s\<equiv> e = s
-                        \<and> loop_update_action_pre e 
-                        \<and> (xs e)!(i e) = 2"
-
-definition dec_highbound_inv1 where 
-"dec_highbound_inv1 e \<equiv> loop_update_action_pre e 
-                        \<and> (xs e)!(i e) = 2
-                        \<and> (xs e)!(high e) = 2
-                        \<and> low_invariant_is_0_Env e"
-
-definition dec_highbound_inv2 where 
-"dec_highbound_inv2 e \<equiv> loop_update_action_pre e 
-                        \<and> (xs e)!(i e) = 2
-                        \<and> (xs e)!(high e) = 2
-                        \<and> invariant_low_to_j_is_1_Env e"
-
-definition dec_highbound_inv3 where 
-"dec_highbound_inv3 e \<equiv> loop_update_action_pre e 
-                        \<and> (xs e)!(i e) = 2
-                        \<and> (xs e)!(high e) = 2
-                        \<and> high_invariant_is_2_Env e"
-
-definition inc_index_pre:: "env \<Rightarrow> env \<Rightarrow> bool" where 
-"inc_index_pre e s \<equiv> e = s 
-                      \<and> loop_update_action_pre e
-                      \<and> (xs e)!(i e) = 1"
-
-definition inc_index_inv1:: "env \<Rightarrow> bool" where 
-"inc_index_inv1 e \<equiv> loop_update_action_pre e
-                    \<and> (xs e)!(i e) = 1
-                    \<and> low_invariant_is_0_Env e"
-
-definition inc_index_inv2:: "env \<Rightarrow> bool" where 
-"inc_index_inv2 e \<equiv> loop_update_action_pre e
-                    \<and> (xs e)!(i e) = 1
-                    \<and> invariant_low_to_j_is_1_Env e"
-
-definition inc_index_inv3:: "env \<Rightarrow> bool" where
-"inc_index_inv3 e \<equiv> loop_update_action_pre e
-                    \<and> (xs e)!(i e) = 1
-                    \<and> high_invariant_is_2_Env e"
-
-subsubsection\<open>Post-conditions\<close>
-definition inc_lowbound_post:: "env \<Rightarrow> env \<Rightarrow> bool" where 
-"inc_lowbound_post e e'\<equiv> high e = high e'
-                          \<and> low e < low e'
-                          \<and> loop_update_action_post e e'
-                          \<and> i e < i e'"
-
-definition dec_highbound_post where 
-"dec_highbound_post e e' \<equiv> length (xs e) > high e' 
-                              \<and> high e = Suc (high e') 
-                              \<and> low e = low e'
-                              \<and> i e = i e'
-                              \<and> (xs e')!(high e') = 2
-                              \<and> loop_update_action_post e e'"
-
-definition inc_index_post:: "env \<Rightarrow> env \<Rightarrow> bool" where 
-"inc_index_post e e' \<equiv> high e = high e' 
-                      \<and> low e = low e'
-                      \<and> Suc(i e) = i e'
-                      \<and> loop_update_action_post e e'"
-
-text\<open>Is it after one iteration of after completion?\<close>
-definition dnfp_post where 
-"dnfp_post e e2 \<equiv> length (xs e) = length (xs e2)
-                  \<and> high e \<ge> high e2
-                  \<and> low e \<le> low e2
-                  \<and> i e \<le> i e2
-                  \<and> high e - i e \<ge> high e2 - i e2
-                  \<and> mset (xs e) = mset (xs e2)"
-
-definition dnfp_inv1:: "env \<Rightarrow> bool" where 
-"dnfp_inv1 e \<equiv> dnfp_pre_aux e
-                \<and> low_invariant_is_0_Env e"
-
-definition dnfp_inv2:: "env \<Rightarrow> bool" where 
-"dnfp_inv2 e \<equiv> dnfp_pre_aux e
-                \<and> invariant_low_to_j_is_1_Env e"
-
-definition dnfp_inv3:: "env \<Rightarrow> bool" where
-"dnfp_inv3 e \<equiv> dnfp_pre_aux e
-                \<and> high_invariant_is_2_Env e"
-
 section\<open>Lemmas\<close>
 subsection\<open>Hoare proofs\<close>
-
-lemma inc_lowbound_spec: "spec (inc_lowbound_pre e) inc_lowbound (GG (inc_lowbound_post e))"
-  unfolding inc_lowbound_pre_def loop_update_action_pre_def GG_def inc_lowbound_post_def loop_update_action_post_def
-  apply(simp_all add: inc_lowbound_def)
-  apply(intro get_rule; intro allI; simp)
-  apply(intro conj_rule_right)
-         apply(intro seq_rule[of _ _ "(\<lambda>_ y. high e = high y)"])
-          apply (simp add: spec_def put_def put_state_def swap_def get_state_def xs_Env_def i_Env_def)
-  apply(intro allI; simp)
-         apply(intro get_rule; intro allI)
-         apply (intro seq_rule[of _ _ "(\<lambda>_ y. high e = high y)"])
-          apply (simp add: spec_def put_def put_state_def swap_def get_state_def i_Env_def)
-          apply (simp add: spec_def put_def get_def return_def put_state_def swap_def get_state_def low_Env_def)
-  apply (intro seq_rule[of _ _ "(\<lambda>_ y. low e = low y)"])
-          apply (simp add: spec_def put_def put_state_def swap_def get_state_def xs_Env_def i_Env_def)
-        apply(intro allI; simp)
-        apply(intro get_rule; intro allI)
-        apply(intro seq_rule[of _ _ "(\<lambda>_ y. low e = low y)"])
-          apply (simp add: spec_def put_def put_state_def swap_def get_state_def i_Env_def)
-        apply(intro allI; simp)
-        apply(intro get_rule; intro allI)
-        apply(simp add: spec_def put_def get_state_def put_state_def low_Env_def)
-       apply (intro seq_rule[of _ _ "(\<lambda>_ y. length (xs e) = length (xs y))"])
-        apply (simp add: spec_def put_def put_state_def swap_def get_state_def xs_Env_def i_Env_def)
-       apply(intro allI)
-  apply(intro get_rule; intro allI; simp)
-       apply (intro seq_rule[of _ _ "(\<lambda>_ y. length (xs e) = length (xs y))"])
-        apply (simp add: spec_def put_def put_state_def swap_def get_state_def i_Env_def)
-       apply(intro allI; simp)
-       apply(intro get_rule; intro allI)
-       apply(simp add: spec_def put_def get_state_def put_state_def low_Env_def)
-      apply (intro seq_rule[of _ _ "(\<lambda>_ y. high y = high e)"])
-       apply (simp add: spec_def put_def put_state_def swap_def get_state_def xs_Env_def i_Env_def)
-       apply(intro allI; simp)
-       apply(intro get_rule; intro allI)
-  apply (intro seq_rule[of _ _ "(\<lambda>_ y. high y = high e)"])
-       apply (simp add: spec_def put_def put_state_def swap_def get_state_def i_Env_def)
-      apply(intro allI; simp)
-      apply(intro get_rule; intro allI)
-      apply(simp add: spec_def put_def get_state_def put_state_def low_Env_def)
-     apply (intro seq_rule[of _ _ "(\<lambda>_ y. low y = low e)"])
-      apply (simp add: spec_def put_def put_state_def swap_def get_state_def xs_Env_def i_Env_def)
-     apply(intro allI; simp)
-     apply(intro get_rule; intro allI)
-     apply (intro seq_rule[of _ _ "(\<lambda>_ y. low y = low e)"])
-      apply (simp add: spec_def put_def put_state_def swap_def get_state_def i_Env_def)
-     apply(intro allI; simp)
-     apply(intro get_rule; intro allI)
-     apply(simp add: spec_def put_def get_state_def put_state_def low_Env_def)
-     apply (intro seq_rule[of _ _ "(\<lambda>_ y. i y = i e)"])
-     apply (simp add: spec_def put_def put_state_def swap_def get_state_def xs_Env_def i_Env_def)
-    apply(intro allI; simp)
-    apply(intro get_rule; intro allI)
-     apply (intro seq_rule[of _ _ "(\<lambda>_ y. i y > i e)"])
-     apply (simp add: spec_def put_def put_state_def swap_def get_state_def i_Env_def)
-    apply(intro allI; simp)
-    apply(intro get_rule; intro allI)
-    apply(simp add: spec_def put_def get_state_def put_state_def low_Env_def)
-   apply (intro seq_rule[of _ _ "(\<lambda>_ y. i y < high y \<and> i y = i e \<and> high y = high e)"])
-    apply (simp add: spec_def put_def put_state_def swap_def get_state_def xs_Env_def i_Env_def)
-   apply(intro allI; simp)
-   apply(intro get_rule; intro allI)
-   apply (intro seq_rule[of _ _ "(\<lambda>_ y. high y - i y < high e - i e)"])
-    apply (simp add: spec_def put_def put_state_def swap_def get_state_def i_Env_def)
-    apply (linarith)
-   apply(intro allI; simp)
-   apply(intro get_rule; intro allI)
-   apply(simp add: spec_def put_def get_state_def put_state_def low_Env_def)
-   apply (intro seq_rule[of _ _ "(\<lambda>x y. i e = i y)"])
-   apply (simp add: spec_def put_def put_state_def swap_def get_state_def xs_Env_def i_Env_def)
-   apply(intro allI; simp)
-   apply(intro get_rule; intro allI)
-   apply (intro seq_rule[of _ _ "(\<lambda>x y. i e < i y)"])
-   apply (simp add: spec_def put_def put_state_def swap_def get_state_def i_Env_def)
-   apply(intro allI; simp)
-   apply(intro get_rule; intro allI)
-  by(simp add: spec_def put_def get_state_def put_state_def low_Env_def)
-
-subsubsection\<open>Invariants\<close>
-lemma inc_lowbound_invariantRed: "spec inc_lowbound_inv1 inc_lowbound (GG low_invariant_is_0_Env)"
-  unfolding inc_lowbound_inv1_def loop_update_action_pre_def  GG_def low_invariant_is_0_Env_def
-  apply(simp_all add: inc_lowbound_def)
-  apply(intro get_rule; intro allI; simp)
-  apply(intro seq_rule[of _ _ "(\<lambda>x e. xs e ! low e = 0 \<and>  (\<forall>x<low e. xs e ! x = 0))"])
-   apply (simp add: spec_def put_def put_state_def swap_def get_state_def xs_Env_def)
-  apply(intro allI; simp)
-  apply(intro get_rule; intro allI)
-  apply(intro seq_rule[of _ _ "(\<lambda>x e. xs e ! low e = 0 \<and> (\<forall>x<low e. xs e ! x = 0))"])
-   apply (simp add: spec_def put_def put_state_def get_state_def i_Env_def)
-  apply(intro allI; simp)
-  apply(intro get_rule; intro allI)
-   apply (simp add: spec_def put_def put_state_def get_state_def low_Env_def)
-  using less_antisym by blast
-
-lemma inc_lowbound_invariantWhite: "spec inc_lowbound_inv2  inc_lowbound (GG invariant_low_to_j_is_1_Env)"
-  unfolding inc_lowbound_inv2_def loop_update_action_pre_def  GG_def invariant_low_to_j_is_1_Env_def
-  apply(simp_all add: inc_lowbound_def)
-  apply(intro get_rule; intro allI; simp)
-   apply (simp add: spec_def put_def put_state_def  get_state_def xs_Env_def swap_def get_def i_Env_def low_Env_def return_def)
-   apply(intro allI)
-  by (simp add: nth_list_update)
-
-lemma inc_lowbound_invariantBlue: "spec inc_lowbound_inv3  inc_lowbound (GG high_invariant_is_2_Env)"
-  unfolding inc_lowbound_inv3_def loop_update_action_pre_def  GG_def high_invariant_is_2_Env_def
-  apply(simp_all add: inc_lowbound_def)
-  apply(intro get_rule; intro allI; simp)
-  apply(intro seq_rule[of _ _ "(\<lambda>x e. \<forall>x \<ge> high e. xs e ! x = 2)"])
-   apply (simp add: spec_def put_def put_state_def swap_def get_state_def xs_Env_def)
-  apply(intro allI; simp)
-  apply(intro get_rule; intro allI)
-  apply(intro seq_rule[of _ _ "(\<lambda>x e. \<forall>x \<ge> high e. xs e ! x = 2)"])
-   apply (simp add: spec_def put_def put_state_def get_state_def i_Env_def)
-  apply(intro allI; simp)
-  apply(intro get_rule; intro allI)
-  by (simp add: spec_def put_def put_state_def get_state_def low_Env_def)
-
-definition inc_lowbound_inv :: "env \<Rightarrow> bool" where
-"inc_lowbound_inv s \<equiv> (inc_lowbound_inv3 s \<and> inc_lowbound_inv2 s \<and> inc_lowbound_inv1 s)"
-
-lemma inc_lowbound_invariants: "spec inc_lowbound_inv  inc_lowbound (GG invariants_Env)"
-  by (metis (mono_tags, lifting) GG_def inc_lowbound_inv_def  inc_lowbound_invariantBlue inc_lowbound_invariantRed inc_lowbound_invariantWhite invariants_Env_def spec_def split_def)
-
-subsection\<open>Dec_highbound Invariants\<close>                                          
-lemma dec_highbound_spec: "spec (dec_highbound_pre e) dec_highbound (GG (dec_highbound_post e))"
-  unfolding dec_highbound_pre_def loop_update_action_pre_def GG_def dec_highbound_post_def loop_update_action_post_def
-  apply(simp_all add: dec_highbound_def)
-  apply(intro get_rule; intro allI; simp)
-  apply(intro conj_rule_right)
-   apply(intro seq_rule[of _ _ "(\<lambda>_ y. high y < length (xs e))"])
-        apply (simp add: spec_def put_def put_state_def get_state_def high_Env_def)
-           apply(linarith)
-           apply(intro allI; simp)
-           apply(intro get_rule; intro allI; simp)
-           apply (simp add: spec_def put_def put_state_def get_state_def xs_Env_def)
-           apply (intro seq_rule[of _ _ "(\<lambda>_ y. (xs e)!(i e) = 2 \<and> (high e = Suc (high y)))"])
-           apply (simp add: spec_def put_def put_state_def get_state_def high_Env_def)
-           apply(intro allI; simp)
-           apply(intro get_rule; intro allI; simp)
-           apply (simp add: spec_def put_def put_state_def get_state_def xs_Env_def)
-          apply(intro seq_rule[of _ _ "(\<lambda>_ y.(xs e)!(i e) = 2 \<and> low e = low y)"])
-           apply (simp add: spec_def put_def put_state_def get_state_def high_Env_def)
-           apply(intro allI; simp)
-          apply(intro get_rule; intro allI; simp)
-             apply (simp add: spec_def put_def put_state_def get_state_def xs_Env_def)
-        apply(intro seq_rule[of _ _ "(\<lambda>_ y. i e = i y \<and> i e < high e \<and> high e \<le> length (xs e))"])
-             apply (simp add: spec_def put_def put_state_def get_state_def high_Env_def)
-           apply(intro allI; simp)
-         apply(intro get_rule; intro allI; simp)
-        apply (simp add: spec_def put_def put_state_def get_state_def xs_Env_def)
-       apply(intro seq_rule[of _ _ "(\<lambda>_ y. i e < high e \<and> high y + 1 = high e \<and> xs e ! i e = 2 \<and> xs e = xs y \<and> i e = i y \<and> high e \<le> length (xs e))"])         
-       apply (simp add: spec_def put_def put_state_def get_state_def high_Env_def)
-        apply(intro allI; simp)
-       apply(intro get_rule; intro allI; simp)
-       apply (simp add: spec_def put_def put_state_def get_state_def xs_Env_def swap_def)
-         apply(intro allI)
-       apply auto[1]
-      apply(intro seq_rule[of _ _ "(\<lambda>_ y. length (xs e) = length (xs y))"])
-      apply (simp add: spec_def put_def put_state_def get_state_def high_Env_def)
-       apply(intro allI; simp)
-       apply(intro get_rule; intro allI; simp)
-       apply (simp add: spec_def put_def put_state_def get_state_def xs_Env_def swap_def)
-      apply(intro seq_rule[of _ _ "(\<lambda>_ y. high y < high e)"])
-      apply (simp add: spec_def put_def put_state_def get_state_def high_Env_def)
-       apply(intro allI; simp)
-      apply(intro get_rule; intro allI; simp)
-      apply (simp add: spec_def put_def put_state_def get_state_def xs_Env_def)
-     apply(intro seq_rule[of _ _ "(\<lambda>_ y. high y < high e \<and> low e = low y)"])
-      apply (simp add: spec_def put_def put_state_def get_state_def high_Env_def)
-       apply(intro allI; simp)
-      apply(intro get_rule; intro allI; simp)
-      apply (simp add: spec_def put_def put_state_def get_state_def xs_Env_def)
-     apply(intro seq_rule[of _ _ "(\<lambda>_ y. i e = i y \<and> high y < high e)"])
-      apply (simp add: spec_def put_def put_state_def get_state_def high_Env_def)
-       apply(intro allI; simp)
-      apply(intro get_rule; intro allI; simp)
-      apply (simp add: spec_def put_def put_state_def get_state_def xs_Env_def)
-     apply(intro seq_rule[of _ _ "(\<lambda>_ y. i e = i y \<and> i e < high e \<and> high y < high e)"])
-      apply (simp add: spec_def put_def put_state_def get_state_def high_Env_def)
-       apply(intro allI; simp)
-   apply(intro get_rule; intro allI; simp)
-   apply (simp add: spec_def put_def put_state_def get_state_def xs_Env_def)
-   apply(intro allI)
-  by(linarith)
-
-subsubsection\<open>Invariants\<close>
-lemma dec_highbound_invariantRed: "spec dec_highbound_inv1 dec_highbound (GG low_invariant_is_0_Env)"
-    unfolding dec_highbound_inv1_def loop_update_action_pre_def GG_def low_invariant_is_0_Env_def
-    apply(simp_all add: dec_highbound_def)
-    apply(intro get_rule; intro allI; simp)
-    apply(intro seq_rule[of _ _ "(\<lambda>_ e. (\<forall>x < low e. xs e ! x = 0) \<and> low e \<le> i e \<and> high e \<ge> i e \<and> length (xs e) > high e)"])
-     apply (simp add: spec_def put_def put_state_def get_state_def high_Env_def swap_def)
-    apply(linarith)
-     apply(intro allI; simp)
-    apply(intro get_rule;intro allI; simp)
-    by (simp add: spec_def put_def put_state_def get_state_def xs_Env_def swap_def)
-
-lemma dec_highbound_invariantWhite: "spec dec_highbound_inv2 dec_highbound (GG invariant_low_to_j_is_1_Env)"
-    unfolding dec_highbound_inv2_def loop_update_action_pre_def GG_def invariant_low_to_j_is_1_Env_def
-    apply(simp_all add: dec_highbound_def)
-        apply(intro get_rule; intro allI; simp)
-    apply(intro seq_rule[of _ _ "(\<lambda>x e. low e \<le> i e \<and> high e \<ge> i e \<and> length (xs e) > high e \<and> (\<forall>x. low e \<le> x \<and> x < i e \<longrightarrow> xs e ! x = Suc 0))"])
-     apply (simp add: spec_def put_def put_state_def get_state_def high_Env_def swap_def)
-    apply linarith
-     apply(intro allI; simp)
-    apply(intro get_rule;intro allI; simp)
-    by (simp add: spec_def put_def put_state_def get_state_def xs_Env_def swap_def)
-
-lemma dec_highbound_invariantBlue: "spec dec_highbound_inv3 dec_highbound (GG high_invariant_is_2_Env)"
-    unfolding dec_highbound_inv3_def loop_update_action_pre_def GG_def high_invariant_is_2_Env_def
-    apply(simp_all add: dec_highbound_def)
-    apply(intro get_rule; intro allI; simp)
-    (*apply(intro seq_rule[of _ _ "(\<lambda>x e. \<forall>x > high e. xs e ! x = 2)"])*)
-     apply (simp add: spec_def put_def put_state_def get_state_def high_Env_def xs_Env_def swap_def get_def return_def)
-    apply(intro allI)
-    by (smt Suc_leI Suc_pred diff_is_0_eq' leD le_eq_less_or_eq length_list_update less_imp_diff_less nth_list_update nth_list_update_neq)
-
-definition dec_highbound_inv :: "env \<Rightarrow> bool" where
-"dec_highbound_inv s \<equiv> (dec_highbound_inv3 s \<and> dec_highbound_inv2 s \<and> dec_highbound_inv1 s)"
-
-lemma dec_highbound_invariants: "spec dec_highbound_inv dec_highbound (GG invariants_Env)"
-  by (metis (mono_tags, lifting) GG_def dec_highbound_inv_def dec_highbound_invariantBlue dec_highbound_invariantRed dec_highbound_invariantWhite invariants_Env_def spec_def split_def)
-
-subsection\<open>Inc_index Invariants\<close>
-lemma inc_index_spec: "spec (inc_index_pre e) inc_index (GG (inc_index_post e))"
-  unfolding inc_index_pre_def loop_update_action_pre_def GG_def inc_index_post_def loop_update_action_post_def
-  apply(simp_all add: inc_index_def)
-  apply(intro get_rule; intro allI;simp)
-  apply(intro conj_rule_right)
-  apply (simp_all add: spec_def put_def put_state_def get_state_def i_Env_def)
-  by linarith
-
-subsubsection\<open>Invariants\<close>
-lemma inc_index_invariantRed: "spec inc_index_inv1 inc_index (GG low_invariant_is_0_Env)"
-  unfolding inc_index_inv1_def loop_update_action_pre_def  GG_def low_invariant_is_0_Env_def
-  apply(simp_all add: inc_index_def)
-  apply(intro get_rule; intro allI; simp)
-  by (simp add: spec_def i_Env_def put_def get_state_def put_state_def)
-
-lemma inc_index_invariantWhite: "spec inc_index_inv2 inc_index (GG invariant_low_to_j_is_1_Env)"
-  unfolding inc_index_inv2_def loop_update_action_pre_def  GG_def invariant_low_to_j_is_1_Env_def
-  apply(simp_all add: inc_index_def)
-  apply(intro get_rule; intro allI; simp)
-  apply (simp add: spec_def i_Env_def put_def get_state_def put_state_def)
-  using less_SucE by blast
-
-lemma inc_index_invariantBlue: "spec inc_index_inv3 inc_index (GG high_invariant_is_2_Env)"
-  unfolding inc_index_inv3_def loop_update_action_pre_def  GG_def high_invariant_is_2_Env_def
-  apply(simp_all add: inc_index_def)
-  apply(intro get_rule; intro allI; simp)
-  by (simp add: spec_def i_Env_def put_def get_state_def put_state_def)
-
-definition inc_index_inv :: "env \<Rightarrow> bool" where
-"inc_index_inv s \<equiv> (inc_index_inv3 s \<and> inc_index_inv2 s \<and> inc_index_inv1 s)"
-
-lemma inc_index_invariants: "spec inc_index_inv inc_index (GG invariants_Env)"
-  by (metis (mono_tags, lifting) GG_def inc_index_inv_def inc_index_invariantBlue inc_index_invariantRed inc_index_invariantWhite invariants_Env_def spec_def split_def)
 
 subsection\<open>Loop update action\<close>
 lemma loop_update_action_spec: "spec (loop_update_action_pre_aux e) loop_update_action (GG (loop_update_action_post e))"
@@ -746,11 +193,13 @@ lemma loop_update_action_invariantBlue: "spec loop_update_action_inv3 loop_updat
    apply (intro cond_rule)
      apply(simp add: inc_lowbound_def) 
      apply(intro get_rule;intro allI; simp)
-  apply(intro seq_rule[of _ _ "(\<lambda>x e. \<forall>x \<ge> high e. xs e ! x = 2)"])
+  apply(intro seq_rule[of _ _ "(\<lambda>x e. \<forall>x. x \<ge> high e \<and> x < length (xs y) \<longrightarrow> xs e ! x = 2)"])
    apply (simp add: spec_def put_def put_state_def swap_def get_state_def xs_Env_def)
-  apply(intro allI; simp)
+   sledgehammer
+   defer
+      apply(intro allI; simp)
   apply(intro get_rule; intro allI)
-  apply(intro seq_rule[of _ _ "(\<lambda>x e. \<forall>x \<ge> high e. xs e ! x = 2)"])
+  apply(intro seq_rule[of _ _ "(\<lambda>x e. \<forall>x. x \<ge> high e \<and> x < length (xs y) \<longrightarrow> xs e ! x = 2)"])
    apply (simp add: spec_def put_def put_state_def get_state_def i_Env_def)
   apply(intro allI; simp)
   apply(intro get_rule; intro allI)
@@ -767,17 +216,13 @@ lemma loop_update_action_invariantBlue: "spec loop_update_action_inv3 loop_updat
 definition loop_update_action_inv :: "env \<Rightarrow> bool" where
 "loop_update_action_inv s \<equiv> (loop_update_action_inv3 s \<and> loop_update_action_inv2 s \<and> loop_update_action_inv1 s)"
 
-
 lemma loop_update_action_invariants: "spec loop_update_action_inv loop_update_action (GG invariants_Env)"
   by (metis (mono_tags, lifting) GG_def loop_update_action_inv_def loop_update_action_invariantBlue loop_update_action_invariantRed loop_update_action_invariantWhite invariants_Env_def spec_def split_def)
-
 
 lemma dnfp_aux1: "spec (\<lambda>y. length (xs e) = length (xs y)) (dnfp_mon v) (\<lambda>x y. length (xs e) = length (xs y))"
   apply(induction v rule: dnfp_mon.induct)
     apply(simp add: spec_def)
     apply (simp add: skip_def)
-    apply(simp add: spec_def)
-   apply (simp add: skip_def)
   apply(simp only: caseN)
   apply(intro get_rule; intro allI; clarify)
   apply(intro cond_rule)
@@ -814,8 +259,6 @@ lemma dnfp_aux2: "spec (\<lambda>y. high y \<le> high e) (dnfp_mon v) (\<lambda>
   apply(induction v rule: dnfp_mon.induct)
     apply(simp add: spec_def)
     apply (simp add: skip_def)
-    apply(simp add: spec_def)
-   apply (simp add: skip_def)
   apply(simp only: caseN)
   apply(intro get_rule; intro allI; clarify)
   apply(intro cond_rule)
@@ -853,8 +296,6 @@ lemma dnfp_aux3: "spec (\<lambda>y. low e \<le> low y) (dnfp_mon v) (\<lambda>x 
   apply(induction v rule: dnfp_mon.induct)
     apply(simp add: spec_def)
     apply (simp add: skip_def)
-    apply(simp add: spec_def)
-   apply (simp add: skip_def)
   apply(simp only: caseN)
   apply(intro get_rule; intro allI; clarify)
   apply(intro cond_rule)
@@ -891,8 +332,6 @@ lemma dnfp_aux4: "spec (\<lambda>y. i e \<le> i y) (dnfp_mon v) (\<lambda>x y. i
   apply(induction v rule: dnfp_mon.induct)
     apply(simp add: spec_def)
     apply (simp add: skip_def)
-    apply(simp add: spec_def)
-   apply (simp add: skip_def)
   apply(simp only: caseN)
   apply(intro get_rule; intro allI; clarify)
   apply(intro cond_rule)
@@ -929,8 +368,6 @@ lemma dnfp_aux5: "spec (\<lambda>y. high y - i y \<le> high e - i e) (dnfp_mon v
   apply(induction v rule: dnfp_mon.induct)
     apply(simp add: spec_def)
     apply (simp add: skip_def)
-    apply(simp add: spec_def)
-   apply (simp add: skip_def)
   apply(simp only: caseN)
   apply(intro get_rule; intro allI; clarify)
   apply(intro cond_rule)
@@ -970,8 +407,6 @@ lemma dnfp_aux6: "spec (\<lambda>y. mset (xs e) = mset (xs y)) (dnfp_mon v) (\<l
   apply(induction v rule: dnfp_mon.induct)
     apply(simp add: spec_def)
     apply (simp add: skip_def)
-    apply(simp add: spec_def)
-   apply (simp add: skip_def)
   apply(simp only: caseN)
   apply(intro get_rule; intro allI; clarify)
   apply(intro cond_rule)
@@ -1007,11 +442,9 @@ lemma dnfp_aux6: "spec (\<lambda>y. mset (xs e) = mset (xs y)) (dnfp_mon v) (\<l
   by (simp add: skip_def)
 
 subsection\<open>DNFP proof\<close>
-lemma dnfp_prepost: "spec (dnfp_pre e) (dnfp_mon n) (GG (dnfp_post e))"
+lemma dnfp_prepost: "spec (dnfp_pre n e) (dnfp_mon n) (GG (dnfp_post n e))"
   apply(induction rule: dnfp_mon.induct)
   unfolding dnfp_pre_def  GG_def dnfp_post_def
-    apply(simp add: spec_def)
-    apply (simp add: skip_def)
     apply(simp add: spec_def)
    apply (simp add: skip_def)
   apply(intro conj_rule_right; simp only: caseN)
@@ -1208,106 +641,88 @@ definition sorted_array :: "env \<Rightarrow> bool" where
   "sorted_array e \<equiv> invariants_Env e 
                   \<and> set(xs e) = {0,1,2}
                   \<and> low e \<le> i e
-                  \<and> i e \<le> high e
+                  \<and> i e = high e
                   \<and> high e \<le> length (xs e)"
-
-definition sorted_array_aux1 :: "env \<Rightarrow> bool" where
-  "sorted_array_aux1 e \<equiv> invariants_Env e 
-                  \<and> set(xs e) \<subseteq> {0}"
-
-lemma sorted_aux1: "\<lbrakk>sorted_array_aux1 e\<rbrakk> \<Longrightarrow> sorted (xs e)"
-  unfolding sorted_array_aux1_def invariants_Env_def high_invariant_is_2_Env_def invariant_low_to_j_is_1_Env_def low_invariant_is_0_Env_def
-  by (smt eq_iff le_numeral_extra(1) less_trans list.size(3) nth_mem set_empty singletonD sorted01 sorted_iff_nth_mono_less subset_singleton_iff)
-
-definition sorted_array_aux2 :: "env \<Rightarrow> bool" where
-  "sorted_array_aux2 e \<equiv> invariants_Env e 
-                  \<and> set(xs e) \<subseteq> {1}
-                  \<and> low e \<le> i e
-                  \<and> i e \<le> high e
-                  \<and> high e \<le> length (xs e)"
-
-lemma sorted_aux2: "\<lbrakk>sorted_array_aux2 e\<rbrakk> \<Longrightarrow> sorted (xs e)"
-  unfolding sorted_array_aux2_def invariants_Env_def high_invariant_is_2_Env_def invariant_low_to_j_is_1_Env_def low_invariant_is_0_Env_def
-  by (smt eq_iff le_numeral_extra(1) less_trans list.size(3) nth_mem set_empty singletonD sorted01 sorted_iff_nth_mono_less subset_singleton_iff)
-
-definition sorted_array_aux3 :: "env \<Rightarrow> bool" where
-  "sorted_array_aux3 e \<equiv> invariants_Env e 
-                  \<and> set(xs e) \<subseteq> {2}"
-
-lemma sorted_aux3: "\<lbrakk>sorted_array_aux3 e\<rbrakk> \<Longrightarrow> sorted (xs e)"
-  unfolding sorted_array_aux3_def invariants_Env_def high_invariant_is_2_Env_def invariant_low_to_j_is_1_Env_def low_invariant_is_0_Env_def
-  by (smt eq_iff le_numeral_extra(1) less_trans list.size(3) nth_mem set_empty singletonD sorted01 sorted_iff_nth_mono_less subset_singleton_iff)
-
-definition sorted_array_aux4 :: "env \<Rightarrow> bool" where
-  "sorted_array_aux4 e \<equiv> invariants_Env e 
-                  \<and> set(xs e) \<subseteq> {0,1}"
-
-lemma sorted_aux4: "\<lbrakk>sorted_array_aux4 e\<rbrakk> \<Longrightarrow> sorted (xs e)"
-  unfolding sorted_array_aux4_def invariants_Env_def high_invariant_is_2_Env_def invariant_low_to_j_is_1_Env_def low_invariant_is_0_Env_def
-  sorry
-
-definition sorted_array_aux5 :: "env \<Rightarrow> bool" where
-  "sorted_array_aux5 e \<equiv> invariants_Env e 
-                  \<and> set(xs e) \<subseteq> {1,2}"
-
-lemma sorted_aux5: "\<lbrakk>sorted_array_aux5 e\<rbrakk> \<Longrightarrow> sorted (xs e)"
-  unfolding sorted_array_aux5_def invariants_Env_def high_invariant_is_2_Env_def invariant_low_to_j_is_1_Env_def low_invariant_is_0_Env_def
-  sorry
-
-definition sorted_array_aux6 :: "env \<Rightarrow> bool" where
-  "sorted_array_aux6 e \<equiv> invariants_Env e 
-                  \<and> set(xs e) \<subseteq> {0,2}"
-
-lemma sorted_aux6: "\<lbrakk>sorted_array_aux6 e\<rbrakk> \<Longrightarrow> sorted (xs e)"
-  unfolding sorted_array_aux6_def invariants_Env_def high_invariant_is_2_Env_def invariant_low_to_j_is_1_Env_def low_invariant_is_0_Env_def
-  sorry
 
 lemma sorted_aux: "\<lbrakk>sorted_array e\<rbrakk> \<Longrightarrow> sorted (xs e)"
   unfolding sorted_array_def invariants_Env_def high_invariant_is_2_Env_def invariant_low_to_j_is_1_Env_def low_invariant_is_0_Env_def
-  sledgehammer
-  sorry
-
+  by (smt Suc_1 Suc_leD less_le_trans nat_le_linear not_less not_one_le_zero sorted_iff_nth_mono)
+  
 subsubsection\<open>Lemmas\<close>
 lemma dnfp_invariantRed_aux: "spec (\<lambda>e. \<forall>x<low e. xs e ! x = 0) (dnfp_mon v) (\<lambda>x e. \<forall>x<low e. xs e ! x = 0)"
  apply(induction v rule: dnfp_mon.induct)
     apply(simp add: spec_def)
     apply (simp add: skip_def)
-    apply(simp add: spec_def)
-   apply (simp add: skip_def)
   apply(simp only: caseN)
   apply(intro get_rule; intro allI; clarify)
   apply(intro cond_rule)
   apply(simp add: loop_update_action_def)
   apply(intro get_rule; intro allI; clarify)
-  apply(intro seq_rule[of _ _ "(\<lambda>x y. \<forall>x<low e. xs e ! x = 0)"])
+  apply(intro seq_rule[of _ _ "(\<lambda>x e. (\<forall>x<low e. xs e ! x = 0))"])
   apply(intro cond_rule)
   apply(simp add: inc_lowbound_def)
-     apply (intro get_rule; intro allI; simp)
-  apply(intro seq_rule[of _ _ "(\<lambda>x e. (\<forall>x<low e. xs e ! x = 0))"])
+      apply (intro get_rule; intro allI; simp)
+  apply(intro seq_rule[of _ _ "(\<lambda>x e. xs e ! low e = 0 \<and> (\<forall>x<low e. xs e ! x = 0))"])
        apply (simp add: spec_def put_def put_state_def swap_def get_state_def xs_Env_def)
+    (*Look here*)
   apply(intro allI)
   defer
        apply(intro allI; simp)
   apply(intro get_rule; intro allI)
   apply(intro seq_rule[of _ _ "(\<lambda>x e. xs e ! low e = 0 \<and> (\<forall>x<low e. xs e ! x = 0))"])
-   apply (simp add: spec_def put_def put_state_def get_state_def i_Env_def)
+        apply (simp add: spec_def put_def put_state_def get_state_def i_Env_def)
   apply(intro allI; simp)
   apply(intro get_rule; intro allI)
-     apply (simp add: spec_def put_def put_state_def get_state_def low_Env_def)
-   using less_antisym apply blast
+       apply (simp add: spec_def put_def put_state_def get_state_def low_Env_def)
+  apply (simp add: less_Suc_eq)
      apply(simp add: dec_highbound_def)
      apply (intro get_rule; intro allI; simp)
-      apply(intro seq_rule[of _ _ "(\<lambda>x e. (\<forall>x<low e. xs e ! x = 0) \<and> high e \<le> length (xs e) \<and> high e \<ge> i e \<and> low e \<le> i e)"]) 
+      apply(intro seq_rule[of _ _ "(\<lambda>x e. low e \<le> i e \<and> i e \<le> high e \<and> (\<forall>x<low e. xs e ! x = 0))"]) 
        apply (simp add: spec_def get_def put_def get_state_def put_state_def high_Env_def)
-       apply(linarith)
+  apply (metis Suc_pred le0 le_less_trans less_Suc_eq_le not_less)
       apply(intro allI; simp)
      apply (intro get_rule; intro allI; simp)
       apply (simp add: spec_def get_def put_def get_state_def put_state_def xs_Env_def swap_def)
      apply(simp add: inc_index_def)
      apply (intro get_rule; intro allI; simp)
+     apply (simp add: spec_def get_def put_def get_state_def put_state_def i_Env_def)
+    apply(intro allI; simp)
+  apply blast
+    apply(simp add: spec_def)
+  apply(simp add: skip_def)
   sorry
 
 lemma dnfp_invariantWhite_aux: "spec (\<lambda>e. \<forall>x. low e \<le> x \<and> x < i e \<longrightarrow> xs e ! x = Suc 0) (dnfp_mon v) (\<lambda>x e. \<forall>x. low e \<le> x \<and> x < i e \<longrightarrow> xs e ! x = Suc 0)"
+ apply(induction v rule: dnfp_mon.induct)
+    apply(simp add: spec_def)
+    apply (simp add: skip_def)
+  apply(simp only: caseN)
+  apply(intro get_rule; intro allI; clarify)
+  apply(intro cond_rule)
+  apply(simp add: loop_update_action_def)
+  apply(intro get_rule; intro allI; clarify)
+  apply(intro seq_rule[of _ _ "(\<lambda>_ e. i e \<ge> low e \<and> high e \<ge> i e \<and> (\<forall>x. low e \<le> x \<and> x < i e \<longrightarrow> xs e ! x = Suc 0))"])
+  apply(intro cond_rule)
+  apply(simp add: inc_lowbound_def)
+     apply (intro get_rule; intro allI; simp)
+   apply (simp add: spec_def put_def put_state_def  get_state_def xs_Env_def swap_def get_def i_Env_def low_Env_def return_def run_state_def)
+      apply(intro allI)
+      apply (simp add: nth_list_update)
+  defer
+     apply(simp add: dec_highbound_def)
+        apply(intro get_rule; intro allI; simp)
+    apply(intro seq_rule[of _ _ "(\<lambda>x e. low e \<le> i e \<and> high e \<ge> i e \<and> length (xs e) > high e \<and> (\<forall>x. low e \<le> x \<and> x < i e \<longrightarrow> xs e ! x = Suc 0))"])
+       apply (simp add: spec_def put_def put_state_def get_state_def high_Env_def swap_def)
+  sledgehammer
+    apply linarith
+     apply(intro allI; simp)
+    apply(intro get_rule;intro allI; simp)
+       apply (simp add: spec_def put_def put_state_def get_state_def xs_Env_def swap_def)
+  defer
+   apply(simp add: inc_index_def)
+   apply(intro get_rule;intro allI; simp)
+   apply (simp add: spec_def put_def put_state_def get_state_def i_Env_def)
+   apply(intro allI)
   sorry
 
 lemma dnfp_invariantBlue_aux: "spec (\<lambda>e. \<forall>x \<ge> high e. xs e ! x = 2) (dnfp_mon v) (\<lambda>x e. \<forall>x \<ge> high e. xs e ! x = 2)"
@@ -1318,8 +733,6 @@ lemma dnfp_invariantRed: "spec dnfp_inv1 (dnfp_mon n) (GG low_invariant_is_0_Env
   apply(induction n rule: dnfp_mon.induct)
     apply(simp add: spec_def)
     apply(simp add: skip_def)
-    apply(simp add: spec_def)
-   apply(simp add: skip_def)
   apply(simp only: caseN)
    apply(intro get_rule; intro allI; clarify)
   apply(intro cond_rule)
@@ -1361,8 +774,6 @@ lemma dnfp_invariantWhite: "spec dnfp_inv2 (dnfp_mon n) (GG invariant_low_to_j_i
   apply(induction n rule: dnfp_mon.induct)
     apply(simp add: spec_def)
     apply(simp add: skip_def)
-    apply(simp add: spec_def)
-   apply(simp add: skip_def)
   apply(simp only: caseN)
    apply(intro get_rule; intro allI; clarify)
   apply(intro cond_rule)
@@ -1388,7 +799,7 @@ lemma dnfp_invariantWhite: "spec dnfp_inv2 (dnfp_mon n) (GG invariant_low_to_j_i
    apply (simp add: spec_def put_def put_state_def get_state_def i_Env_def)
     apply(intro allI)
     apply (metis Suc_lessI less_SucE)
-  apply(intro allI)
+    apply(intro allI)
    using dnfp_invariantWhite_aux apply blast
     apply(simp add: spec_def)
    by(simp add: skip_def)
@@ -1398,8 +809,6 @@ lemma dnfp_invariantBlue: "spec dnfp_inv3 (dnfp_mon n) (GG high_invariant_is_2_E
   apply(induction n rule: dnfp_mon.induct)
     apply(simp add: spec_def)
     apply(simp add: skip_def)
-    apply(simp add: spec_def)
-   apply(simp add: skip_def)
   apply(simp only: caseN)
    apply(intro get_rule; intro allI; clarify)
   apply(intro cond_rule)
@@ -1422,8 +831,6 @@ lemma dnfp_invariantBlue: "spec dnfp_inv3 (dnfp_mon n) (GG high_invariant_is_2_E
      apply(intro get_rule; intro allI)
      apply (simp add: spec_def put_def put_state_def get_state_def high_Env_def xs_Env_def swap_def get_def return_def run_state_def)
      apply(intro allI)
-  sledgehammer
-   apply (smt One_nat_def Suc_leI Suc_pred le_less length_list_update less_Suc_eq_0_disj less_imp_Suc_add less_le_trans nth_list_update value_must_be_two)
    defer
    apply(simp add: inc_index_def)
     apply(intro get_rule; intro allI; simp)
@@ -1432,6 +839,23 @@ lemma dnfp_invariantBlue: "spec dnfp_inv3 (dnfp_mon n) (GG high_invariant_is_2_E
   apply(simp add: spec_def)
    apply(simp add: skip_def)
    sorry
+
+definition sorted_dnfp_pre where
+ "sorted_dnfp_pre e \<equiv> i e = 0
+                    \<and> low e = 0
+                    \<and> high e = length (xs e)"
+
+lemma sorted_dnfp_aux1: "\<lbrakk>sorted_dnfp_pre e\<rbrakk> \<Longrightarrow> low_invariant_is_0_Env e"
+  unfolding sorted_dnfp_pre_def  low_invariant_is_0_Env_def
+  by simp
+
+lemma sorted_dnfp_aux2: "\<lbrakk>sorted_dnfp_pre e\<rbrakk> \<Longrightarrow> invariant_low_to_j_is_1_Env e"
+  unfolding sorted_dnfp_pre_def  invariant_low_to_j_is_1_Env_def
+  by simp
+
+lemma sorted_dnfp_aux3: "\<lbrakk>sorted_dnfp_pre e\<rbrakk> \<Longrightarrow> high_invariant_is_2_Env e"
+  unfolding sorted_dnfp_pre_def  high_invariant_is_2_Env_def
+  by auto
 
 
 
