Monad_Play Around/DNFP/Dutch_National_Flag_Monad_Definitions.thy
@@ -1,0 +1,291 @@
+theory Dutch_National_Flag_Monad_Definitions
+imports 
+  Main
+  "../State_Monad_HL"
+  "HOL-Library.Multiset"
+begin
+type_synonym 'a array = "'a list"
+  
+section\<open>Monad definitions\<close>
+record env = 
+  high :: "nat"
+  low  :: "nat"
+  i    :: "nat"
+  xs   :: "nat array"
+
+subsection\<open>update functions\<close>
+definition high_Env:: "env \<Rightarrow> nat \<Rightarrow> env" where "high_Env s v = s \<lparr> high := v \<rparr>"
+definition low_Env:: "env \<Rightarrow> nat \<Rightarrow> env" where "low_Env s v = s \<lparr> low := v \<rparr>"
+definition i_Env:: "env \<Rightarrow> nat \<Rightarrow> env" where "i_Env s v = s \<lparr> i := v \<rparr>"
+definition xs_Env:: "env \<Rightarrow> nat array  \<Rightarrow> env" where "xs_Env s v = s \<lparr> xs := v \<rparr>"
+
+theorem put_high_rule: "spec (\<lambda>x. p () (x \<lparr> high := v \<rparr>)) (put high_Env v) p"
+  by (simp add: spec_def put_def get_state_def put_state_def high_Env_def)
+
+theorem put_low_rule: "spec (\<lambda>x. p () (x \<lparr> low := v \<rparr>)) (put low_Env v) p"
+  by (simp add: spec_def put_def get_state_def put_state_def low_Env_def)
+
+theorem put_i_rule: "spec (\<lambda>x. p () (x \<lparr> i := v \<rparr>)) (put i_Env v) p"
+  by (simp add: spec_def put_def get_state_def put_state_def i_Env_def)
+
+theorem put_xs_rule: "spec (\<lambda>x. p () (x \<lparr> xs := v \<rparr>)) (put xs_Env v) p"
+  by (simp add: spec_def put_def get_state_def put_state_def xs_Env_def)
+
+
+definition swap:: "'a array \<Rightarrow> nat \<Rightarrow> nat \<Rightarrow> 'a array" where
+"swap l x y \<equiv> (if x < length l \<and> y < length l then l[x := l!y, y := l!x] else l)"
+
+lemma length_swap: "length(swap l x y) = length l"
+  by(simp add: swap_def)
+
+lemma distinct_swap[simp]:
+  "distinct(swap l x y) = distinct l"
+  by(simp add: swap_def)
+
+lemma mset_swap: "mset (swap l x y) = mset l"
+  by (simp add: swap_def mset_swap)
+
+section\<open>DNFP function definitions\<close>
+definition inc_lowbound where
+"inc_lowbound \<equiv> do{
+                  (l, s, j) \<leftarrow> get (\<lambda>e. (low e, xs e, i e));  
+                  put xs_Env (swap s j l);
+                  j \<leftarrow> get i;                                   
+                  put i_Env (Suc j);
+                  l \<leftarrow> get low;  
+                  put low_Env (Suc l)
+                }"
+
+definition dec_highbound where
+"dec_highbound \<equiv> do{
+                    h \<leftarrow> get high;
+                    put high_Env (h - 1);
+                    (s, j, h) \<leftarrow> get (\<lambda>e. (xs e, i e, high e));
+                    put xs_Env (swap s j h)
+                }"
+
+definition inc_index where
+"inc_index \<equiv> do{
+                  j \<leftarrow> get i;
+                  put i_Env (Suc j)
+                }"
+
+definition loop_update_action where
+"loop_update_action \<equiv> 
+  do{
+    (s, j) \<leftarrow> get (\<lambda>e. (xs e, i e));
+    (if s!j < 1 then do {
+      inc_lowbound
+    } else (if s!j > 1 then do 
+    {
+      dec_highbound
+    }
+   else do {
+      inc_index
+   }))
+  }"
+
+
+definition init_env:: "nat array \<Rightarrow> env" where
+  "init_env l \<equiv> \<lparr>high = (length l),            low = 0,
+                 i = 0,                         xs = l\<rparr>"
+
+definition init_state_env:: "nat array \<Rightarrow> (env, unit) state" where
+  "init_state_env l \<equiv> State (\<lambda>x. ((),init_env l))"
+
+value \<open>snd(run_state (dnfp_mon 5) (init_env [0,2,2,1,2]))\<close>
+value \<open>snd(run_state (dnfp_mon 9) (init_env [0,2,2,0,1,0,2,1,2]))\<close>
+value \<open>snd(run_state (dnfp_mon 3)(init_env [2,1,0]))\<close>
+
+value \<open>sorted(xs(snd(run_state (dnfp_mon 5) (init_env[0,2,2,1,2]))))\<close>
+value \<open>sorted(xs(snd(run_state (dnfp_mon 9) (init_env[0,2,2,0,1,0,2,1,2]))))\<close>
+value \<open>sorted(xs(snd(run_state (dnfp_mon 3) (init_env[2,1,0]))))\<close>
+
+section\<open>Definiton of all the Pre and postconditions\<close>
+
+subsection\<open>The invariants are taken from https://en.wikipedia.org/wiki/Dutch_national_flag_problem\<close>
+definition low_invariant_is_0 where
+"low_invariant_is_0 arr l \<equiv> (\<forall>x. x < l \<longrightarrow> arr!x = 0)"
+
+definition invariant_low_to_j_is_1 where
+"invariant_low_to_j_is_1 arr l j \<equiv> (\<forall>x. (x \<ge> l \<and> x < j) \<longrightarrow> arr!x = 1)"
+
+definition high_invariant_is_2 where
+"high_invariant_is_2 arr h\<equiv> (\<forall>x. x \<ge> h \<longrightarrow> arr!x = 2)"
+
+definition low_invariant_is_0_Env where
+"low_invariant_is_0_Env e \<equiv> (\<forall>x. x < (low e) \<longrightarrow> (xs e)!x = 0)"
+
+definition invariant_low_to_j_is_1_Env where
+"invariant_low_to_j_is_1_Env e \<equiv> (\<forall>x. (x \<ge> (low e) \<and> x < (i e)) \<longrightarrow> (xs e)!x = 1)"
+
+definition high_invariant_is_2_Env where
+"high_invariant_is_2_Env e\<equiv> (\<forall>x. x \<ge> (high e) \<and> x < length (xs e) \<longrightarrow> (xs e)!x = 2)"
+
+definition invariants_Env:: "env \<Rightarrow> bool" where
+"invariants_Env e \<equiv> high_invariant_is_2_Env e
+              \<and> invariant_low_to_j_is_1_Env e
+              \<and> low_invariant_is_0_Env e"
+
+definition invariants where
+"invariants arr l j h\<equiv> low_invariant_is_0 arr l
+              \<and> invariant_low_to_j_is_1 arr l j
+              \<and> high_invariant_is_2 arr h"
+
+text\<open>This can be used in the other pre and post-conditions for the methods inside loop_update_actions\<close>
+
+subsection\<open>Pre- and Postconditions\<close>
+
+subsubsection\<open>Pre-conditions\<close>
+definition dnfp_pre:: "env \<Rightarrow> env \<Rightarrow> bool" where
+"dnfp_pre e s \<equiv> s = e
+              \<and> high e \<ge> i e
+              \<and> i e \<ge> low e 
+              \<and> length (xs e) \<ge> high e
+              \<and> set (xs e) \<subseteq> {1,2,3}"
+
+definition dnfp_pre_aux:: "env \<Rightarrow> bool" where
+"dnfp_pre_aux e \<equiv> 
+              high e \<ge> i e
+              \<and> i e \<ge> low e 
+              \<and> length (xs e) \<ge> high e
+              \<and> set (xs e) \<subseteq> {1,2,3}"
+
+definition loop_update_action_pre:: "env \<Rightarrow> bool" where
+"loop_update_action_pre e \<equiv> high e > i e
+                             \<and> length (xs e) > (Suc 0)
+                             \<and> length (xs e) \<ge> high e
+                             \<and> low e < high e
+                             \<and> low e \<le> i e
+                             \<and> set (xs e) \<subseteq> {0,1,2}"
+
+definition loop_update_action_pre_aux:: "env \<Rightarrow> env \<Rightarrow> bool" where
+"loop_update_action_pre_aux e s \<equiv> s = e
+                              \<and> loop_update_action_pre e"
+
+definition loop_update_action_inv1 where 
+"loop_update_action_inv1 e \<equiv> loop_update_action_pre e 
+                            \<and> low_invariant_is_0_Env e"
+
+definition loop_update_action_inv2 where 
+"loop_update_action_inv2 e \<equiv> loop_update_action_pre e 
+                              \<and> invariant_low_to_j_is_1_Env e"
+
+definition loop_update_action_inv3 where 
+"loop_update_action_inv3 e \<equiv> loop_update_action_pre e 
+                              \<and> high_invariant_is_2_Env e"
+
+definition loop_update_action_post where
+"loop_update_action_post e e' \<equiv> length (xs e) = length (xs e')
+                                \<and> high e \<ge> high e'
+                                \<and> low e \<le> low e'
+                                \<and> i e \<le> i e'
+                                \<and> high e - i e > high e' - i e'"
+
+definition inc_lowbound_pre:: "env \<Rightarrow> env \<Rightarrow> bool" where 
+"inc_lowbound_pre e s \<equiv> s = e
+                        \<and> loop_update_action_pre s
+                        \<and> (xs s)!(i s) < 1"
+
+definition inc_lowbound_inv1 :: "env \<Rightarrow> bool" where
+"inc_lowbound_inv1 s \<equiv> loop_update_action_pre s
+                        \<and> (xs s)!(i s) < 1
+                        \<and> low_invariant_is_0_Env s"
+
+definition inc_lowbound_inv2 :: "env \<Rightarrow> bool" where
+"inc_lowbound_inv2 s \<equiv> loop_update_action_pre s
+                        \<and> (xs s)!(i s) < 1
+                        \<and> invariant_low_to_j_is_1_Env s"
+
+definition inc_lowbound_inv3 :: "env \<Rightarrow> bool" where
+"inc_lowbound_inv3 s \<equiv> loop_update_action_pre s
+                        \<and> (xs s)!(i s) < 1
+                        \<and> high_invariant_is_2_Env s"
+
+definition dec_highbound_pre where 
+"dec_highbound_pre e s\<equiv> e = s
+                        \<and> loop_update_action_pre e 
+                        \<and> (xs e)!(i e) = 2"
+
+definition dec_highbound_inv1 where 
+"dec_highbound_inv1 e \<equiv> loop_update_action_pre e 
+                        \<and> (xs e)!(i e) = 2
+                        \<and> (xs e)!(high e) = 2
+                        \<and> low_invariant_is_0_Env e"
+
+definition dec_highbound_inv2 where 
+"dec_highbound_inv2 e \<equiv> loop_update_action_pre e 
+                        \<and> (xs e)!(i e) = 2
+                        \<and> (xs e)!(high e) = 2
+                        \<and> invariant_low_to_j_is_1_Env e"
+
+definition dec_highbound_inv3 where 
+"dec_highbound_inv3 e \<equiv> loop_update_action_pre e 
+                        \<and> (xs e)!(i e) = 2
+                        \<and> (xs e)!(high e) = 2
+                        \<and> high_invariant_is_2_Env e"
+
+definition inc_index_pre:: "env \<Rightarrow> env \<Rightarrow> bool" where 
+"inc_index_pre e s \<equiv> e = s 
+                      \<and> loop_update_action_pre e
+                      \<and> (xs e)!(i e) = 1"
+
+definition inc_index_inv1:: "env \<Rightarrow> bool" where 
+"inc_index_inv1 e \<equiv> loop_update_action_pre e
+                    \<and> (xs e)!(i e) = 1
+                    \<and> low_invariant_is_0_Env e"
+
+definition inc_index_inv2:: "env \<Rightarrow> bool" where 
+"inc_index_inv2 e \<equiv> loop_update_action_pre e
+                    \<and> (xs e)!(i e) = 1
+                    \<and> invariant_low_to_j_is_1_Env e"
+
+definition inc_index_inv3:: "env \<Rightarrow> bool" where
+"inc_index_inv3 e \<equiv> loop_update_action_pre e
+                    \<and> (xs e)!(i e) = 1
+                    \<and> high_invariant_is_2_Env e"
+
+subsubsection\<open>Post-conditions\<close>
+definition inc_lowbound_post:: "env \<Rightarrow> env \<Rightarrow> bool" where 
+"inc_lowbound_post e e'\<equiv> high e = high e'
+                          \<and> low e < low e'
+                          \<and> loop_update_action_post e e'
+                          \<and> i e < i e'"
+
+definition dec_highbound_post where 
+"dec_highbound_post e e' \<equiv> length (xs e) > high e' 
+                              \<and> high e = Suc (high e') 
+                              \<and> low e = low e'
+                              \<and> i e = i e'
+                              \<and> (xs e')!(high e') = 2
+                              \<and> loop_update_action_post e e'"
+
+definition inc_index_post:: "env \<Rightarrow> env \<Rightarrow> bool" where 
+"inc_index_post e e' \<equiv> high e = high e' 
+                      \<and> low e = low e'
+                      \<and> Suc(i e) = i e'
+                      \<and> loop_update_action_post e e'"
+
+text\<open>Is it after one iteration of after completion?\<close>
+definition dnfp_post where 
+"dnfp_post e e2 \<equiv> length (xs e) = length (xs e2)
+                  \<and> high e \<ge> high e2
+                  \<and> low e \<le> low e2
+                  \<and> i e \<le> i e2
+                  \<and> high e - i e \<ge> high e2 - i e2
+                  \<and> mset (xs e) = mset (xs e2)"
+                  (*\<and> i e2 = high e2*)
+
+definition dnfp_inv1:: "env \<Rightarrow> bool" where 
+"dnfp_inv1 e \<equiv> dnfp_pre_aux e
+                \<and> low_invariant_is_0_Env e"
+
+definition dnfp_inv2:: "env \<Rightarrow> bool" where 
+"dnfp_inv2 e \<equiv> dnfp_pre_aux e
+                \<and> invariant_low_to_j_is_1_Env e"
+
+definition dnfp_inv3:: "env \<Rightarrow> bool" where
+"dnfp_inv3 e \<equiv> dnfp_pre_aux e
+                \<and> high_invariant_is_2_Env e"
+
+end
